test/general/test_infer_returns.c
@@ -1,0 +1,65 @@
+#include <stdint.h>
+#include <stdlib.h>
+#include <stdbool.h>
+#include "../include/PulseMacros.h"
+
+typedef struct _foo{
+int a; 
+int b;
+};
+
+union ab {
+    int a; 
+    bool b;
+};
+
+uint32_t foo(){
+    return 10;
+}
+
+long long foo1(){
+    return 10;
+}
+
+long foo2(){
+    return 10;
+}
+
+int* foo3(){
+    int *x;
+    return x;
+}
+
+uint32_t* foo4(){
+    uint32_t *x;
+    return x;
+}
+
+void foo5(){
+    return;
+}
+
+//Vidush: Should we just fail for all functions 
+//that return a void pointer?
+EXPECT_FAILURE()
+void *foo6(){
+    return NULL;
+}
+
+bool foo7(){
+    return false;
+}
+
+int32_t bar(){
+    return 10;
+}
+
+struct _foo *baz(){
+    return NULL;
+}
+
+ERASED_ARG(s:_)
+REQUIRES(pure (Case_ab_a? s))
+union ab *baz1(union ab *x){
+    return x;
+}
