test/general/test_union.c
@@ -35,5 +35,31 @@ match s.tag with\
 | 1y -> Case_ab_b? s.payload\
 | _ -> false\
 )"
-)                                          
+)
+
+
+
+EXPECT_FAILURE()
+ERASED_ARG(#s : stru_spec)
+REQUIRES(stru_pred foo s)
+ERASED_ARG(s:_)
+REQUIRES(pure (Case_ab_a? s))
+REQUIRES(ab_pred foo.payload s)
+REQUIRES(pure (UInt32.fits (UInt32.v (Case_ab_a?._0 s) + 1)))
+ENSURES(exists* s'. ab_pred foo.payload s')
+ENSURES("exists* (s':stru_spec). stru_pred foo s' ** pure (s' == {tag = s.tag; payload = s.payload})")
+void test_union(struct stru * foo){
+
+  if (foo->tag == 0){
+    foo->payload.a += 1; 
+  }
+  else if (foo->tag == 1){
+    foo->payload.b = !(foo->payload.b);
+  }
+}
+
+
+
+
+
 
