test/snapshots/Test_bool_2.fst
@@ -9,6 +9,7 @@ open Pulse.Lib.C
 
 fn foo
 (p : Int64.t)
+returns Int32.t
 {
 let mut p : Int64.t = p;
 if((int32_to_bool (bool_to_int32 (op_AmpAmp (int64_to_bool (! p)) (int64_to_bool (! p))))))
@@ -19,4 +20,5 @@ else
 {
 ()
 };
+0l;
 }
