test/snapshots/Swap_struct_test_2.fst
@@ -130,10 +130,12 @@ _u32_pair_struct_recover !x;
 }
 
 fn main ()
+returns Int32.t
 {
 let mut x : (ref _u32_pair_struct) = (new_u32_pair_struct ());
 (swap_fields (! x));
 (swap_fields_alt (! x));
 with vx. assert ((x |-> vx) ** _u32_pair_struct_pred vx {first = 0ul; second = 1ul});
 (_u32_pair_struct_free (! x));
+0l;
 }
