test/snapshots/Test_infer_returns.fst
@@ -1,0 +1,187 @@
+module Test_infer_returns
+
+#lang-pulse
+
+open Pulse
+open Pulse.Lib.C
+
+
+
+noeq
+type _foo = {
+a: ref Int32.t;
+b: ref Int32.t;
+}
+
+[@@erasable]
+noeq
+type _foo_spec = {
+a : Int32.t;
+b : Int32.t
+
+}
+
+let _foo_pred ([@@@mkey]x:ref _foo) (s:_foo_spec) : slprop =
+exists* (y: _foo). (x |-> y) **
+(y.a |-> s.a) **
+(y.b |-> s.b)
+
+assume val _foo_spec_default : _foo_spec
+
+assume val _foo_default (_foo_var_spec:_foo_spec) : _foo
+
+ghost
+fn _foo_pack (_foo_var:ref _foo) (#_foo_var_spec:_foo_spec)
+requires _foo_var|-> _foo_default _foo_var_spec
+ensures exists* v. _foo_pred _foo_var v ** pure (v == _foo_var_spec)
+{ admit() }
+
+ghost
+fn _foo_unpack (_foo_var:ref _foo)
+requires exists* v. _foo_pred _foo_var v 
+ensures exists* u. _foo_var |-> u
+{ admit() }
+
+fn _foo_alloc ()
+returns x:ref _foo
+ensures freeable x
+ensures exists* v. _foo_pred x v
+{ admit () }
+
+fn _foo_free (x:ref _foo)
+requires freeable x
+requires exists* v. _foo_pred x v
+{ admit() }
+
+
+ghost fn _foo_explode (x:ref _foo) (#s:_foo_spec)
+requires _foo_pred x s
+ensures exists* (v: _foo). (x |-> v) ** (v.a |-> s.a) ** 
+(v.b |-> s.b)
+
+{unfold _foo_pred}
+
+
+ghost
+fn _foo_recover (x:ref _foo) (#a0 : Int32.t)
+(#a1 : Int32.t)
+
+requires exists* (y: _foo). (x |-> y) ** 
+(y.a |-> a0) **
+(y.b |-> a1)
+ensures exists* w. _foo_pred x w ** pure (w == {a = a0;
+b = a1})
+{fold _foo_pred x ({a = a0;
+b = a1}) }
+
+noeq
+type ab = {
+a: ref Int32.t;
+b: ref bool;
+}
+
+noeq
+type ab_spec = 
+ | Case_ab_a of Int32.t
+ | Case_ab_b of bool
+
+let ab_pred(u : ref ab) (s : ab_spec) : slprop =
+exists* uv. (u |-> uv) **
+begin match s with
+ | Case_ab_a v -> uv.a |-> v
+ | Case_ab_b v -> uv.b |-> v
+end
+
+fn ab_explode (x : ref ab) (#s : ab_spec)
+requires ab_pred x s
+ensures exists* (v : ab). (x |-> v) **
+begin match s with
+ | Case_ab_a w -> v.a |-> w
+ | Case_ab_b w -> v.b |-> w
+end
+{
+unfold ab_pred;
+}
+
+ghost
+fn ab_recover (x : ref ab) (#s : ab_spec)
+requires exists* (v : ab). (x |-> v) **
+begin match s with
+ | Case_ab_a w -> v.a|-> w
+ | Case_ab_b w -> v.b|-> w
+end
+ensures ab_pred x s
+{
+fold (ab_pred x s);
+}
+
+fn foo ()
+returns UInt32.t
+{
+(int32_to_uint32 10l);
+}
+
+fn foo1 ()
+returns Int64.t
+{
+(int32_to_int64 10l);
+}
+
+fn foo2 ()
+returns Int64.t
+{
+(int32_to_int64 10l);
+}
+
+fn foo3 ()
+returns (ref Int32.t)
+{
+let mut x: (ref Int32.t) = witness #_ #_;
+(! x);
+}
+
+fn foo4 ()
+returns (ref UInt32.t)
+{
+let mut x: (ref UInt32.t) = witness #_ #_;
+(! x);
+}
+
+fn foo5 ()
+{
+();
+}
+
+[@@expect_failure]
+fn foo6 ()
+{
+((null #_));
+}
+
+fn foo7 ()
+returns bool
+{
+(int32_to_bool 0l);
+}
+
+fn bar ()
+returns Int32.t
+{
+10l;
+}
+
+fn baz ()
+returns (ref _foo)
+{
+(null #_);
+}
+
+fn baz1
+(x : ( ref ab) )
+(s:_)
+requires pure (Case_ab_a? s)
+returns (ref ab)
+{
+let mut x : (ref ab) = x;
+(! x);
+}
